WIP

src/RawRenamingEquations.v
@@ -1,64 +1,8 @@
-Require Import Label PeanoNat Psatz Ring Compare_dec StrictProp.
+Require Import Label PeanoNat Psatz Ring
+        Compare_dec StrictProp  Setoid Morphisms.
 Require Import Var VarEquations RawRenaming.
 
-(* Properties of raw renaming composition *)
-
-Definition apply_renaming_rhs_var r : var_op 0 1 :=
-  lift_var_op (apply_raw_renaming_var (rhs_raw_renaming r))
-  @ push_var (rhs_push r).
-Arguments apply_renaming_rhs_var r /.
-
-(* TODO: move to var equations *)
-Lemma lift_var_op_compose'
-      {L N M O} (op1 : var_op N M) (op2 : var_op L N)
-      (op3 : var_op O (S L)) :
-  lift_var_op (op1 @ op2) @ op3
-  =v= lift_var_op op1 @ (lift_var_op op2 @ op3).
-Proof.
-  rewrite var_op_associative.
-  rewrite lift_var_op_compose.
-  rewrite <- var_op_associative.
-  easy.
-Qed.
-
-(* TODO: move to var equations *)
-Ltac case_vars_eq v1 v2 :=
-  let Hneql := fresh "Hneql" in
-  change (var_eqb v1 v2)
-    with (if var_dec v1 v2 then true else false);
-  destruct (var_dec v1 v2) as [<-|Hneql]; cbn.
-
-Lemma apply_transpose_push_raw_renaming v r :
-  push_var v
-  @ apply_raw_renaming_var r
-  =v=
-  apply_renaming_rhs_var (transpose_push_raw_renaming v r).
-Proof.
-  generalize dependent v.
-  induction r as [|vl r IHr vr]; intros v; cbn.
-  - simplify_var_ops; easy.
-  - case_vars_eq v vl.
-    + rewrite push_pop_identity'; easy.
-    + rewrite transpose_push_pop' by easy.
-      simplify_var_ops.
-      rewrite <- lift_var_op_compose'.
-      rewrite IHr; cbn; simplify_var_ops.
-      rewrite transpose_swap_lifted'.
-      rewrite transpose_pushes.
-      rewrite swap_swap_identity'.
-      easy.
-Qed.
-
-Lemma apply_compose_raw_renaming r1 r2 :
-  apply_raw_renaming_var (compose_raw_renaming r1 r2)
-  =v= apply_raw_renaming_var r1 @ apply_raw_renaming_var r2.
-Proof.
-  generalize dependent r2.
-  induction r1 as [|vl r1 IHr1 vr]; intros r2; cbn; try easy.
-  rewrite IHr1; simplify_var_ops.
-  rewrite apply_transpose_push_raw_renaming.
-  easy.
-Qed.
+(* Raw renamings form a semigroup *)
 
 Lemma raw_renaming_left_identity r :
   compose_raw_renaming raw_renaming_id r = r.
@@ -145,159 +89,353 @@ Proof.
   generalize dependent v1.
   generalize dependent v2.
   induction r as [|vl r IHr vr]; intros v2 v1; cbn; try easy.
-  case_vars_eq v1 vl.
-  - rewrite transpose_op_reducing_push_pop.
-
-  case_var_zero vo1.
-  - rewrite transpose_push_reducing_push_pop; easy.
-  - rewrite transpose_push_normalized_pushes_cons_push; cbn.
-    case_var_zero vo2.
-    + apply transpose_pushes_squared_right.
-    + rewrite transpose_pushes_reverse_right.
+  case_vars_eq v1 vl as Heq1 Hneq1.
+  - rewrite var_eqb_false by apply irreducible_transposed_1.
+    rewrite reducible_transposed_2 with (v1 := v2) by easy.
+    easy.
+  - case_vars_eq (shift_var v1 v2) vl as Heq2 Hneq2.
+    + apply reducible_transposed_2 in Heq2 as Heq3;
+        reduce_vars.
+      apply transpose_pushes_squared_right.
+    + apply irreducible_transposed_3 in Hneq2 as Hneq3;
+        try easy; reduce_vars.
+      rewrite transpose_pushes_reverse_right.
       rewrite IHr.
-      rewrite transpose_push_push_pop_zero_reverse_right
-        by easy.
-      easy.
+      rewrite transpose_push_push_pop_reverse_right
+        by congruence; easy.
 Qed.
 
-Lemma transpose_push_raw_closing_reverse_middle vo1 vo2 r :
-  unshift_var_opt
-    (transpose_push_raw_closing_push
-       vo1 (transpose_push_raw_closing_raw_closing vo2 r))
-    (transpose_push_raw_closing_push vo2 r)
-  = transpose_push_raw_closing_push
-      (unshift_var_opt vo1 vo2)
-      (transpose_push_raw_closing_raw_closing
-         (shift_var_opt vo2 vo1) r).
+Lemma transpose_push_raw_renaming_reverse_middle v1 v2 r :
+  unshift_var
+    (transpose_push_raw_renaming_push
+       v1 (transpose_push_raw_renaming_raw_renaming v2 r))
+    (transpose_push_raw_renaming_push v2 r)
+  = transpose_push_raw_renaming_push
+      (unshift_var v1 v2)
+      (transpose_push_raw_renaming_raw_renaming
+         (shift_var v2 v1) r).
 Proof.
-  generalize dependent vo1.
-  generalize dependent vo2.
-  induction r as [|vo3 r]; intros vo2 vo1; cbn; try easy.
-  case_var_zero vo2.
-  - rewrite transpose_push_normalized_pushes_cons_push; cbn.
-    rewrite transpose_push_push_zero_left; cbn.
-    rewrite transpose_push_reducing_push_pop; easy.
-  - rewrite transpose_push_normalized_pushes_cons_push; cbn.
-    case_var_zero vo1.
-    + rewrite transpose_pushes_squared_left.
-      destruct vo2; easy.
-    + rewrite transpose_push_normalized_pushes_cons_push;
-        cbn; reduce_var_zero.
+  generalize dependent v1.
+  generalize dependent v2.
+  induction r as [|vl r IHr vr]; intros v2 v1; cbn; try easy.
+  case_vars_eq v2 vl as Heq1 Hneq1.
+  - rewrite var_eqb_false
+      by apply irreducible_transposed_1; cbn.
+    rewrite var_eqb_true
+      by apply transpose_reducible_push_pop.
+    rewrite reducible_transposed_2
+      with (v2 := v2) (v1 := v1) by easy.
+    easy.
+  - case_vars_eq (shift_var v2 v1) vl as Heq2 Hneq2.
+    + apply reducible_transposed_2 in Heq2 as Heq3;
+        reduce_vars.
+      rewrite transpose_pushes_squared_left.
+      rewrite <- transpose_reducible_push_pop.
+      easy.
+    + apply irreducible_transposed_3 in Hneq2 as Hneq3;
+        try easy; reduce_vars.
+      rewrite var_eqb_false
+        by (apply transpose_irreducible_push_pop; easy).
       rewrite transpose_pushes_reverse_middle.
       rewrite IHr.
-      rewrite transpose_push_push_pop_zero_reverse_middle.
-      rewrite transpose_push_raw_closing_reverse_right.
-      rewrite transpose_push_push_pop_zero_reverse_right
-        by easy.
+      rewrite transpose_push_raw_renaming_reverse_right.
+      rewrite transpose_push_push_pop_reverse_middle.
+      rewrite transpose_push_push_pop_reverse_right
+        by congruence.
       easy.
 Qed.
 
-Lemma transpose_push_raw_closing_reverse_left vo1 vo2 r :
-  transpose_push_raw_closing_raw_closing vo1
-    (transpose_push_raw_closing_raw_closing vo2 r)
-  = transpose_push_raw_closing_raw_closing
-      (unshift_var_opt vo1 vo2)
-      (transpose_push_raw_closing_raw_closing
-         (shift_var_opt vo2 vo1) r).
+Lemma transpose_push_raw_renaming_reverse_left v1 v2 r :
+  transpose_push_raw_renaming_raw_renaming v1
+    (transpose_push_raw_renaming_raw_renaming v2 r)
+  = transpose_push_raw_renaming_raw_renaming
+      (unshift_var v1 v2)
+      (transpose_push_raw_renaming_raw_renaming
+         (shift_var v2 v1) r).
 Proof.
-  generalize dependent vo1.
-  generalize dependent vo2.
-  induction r as [|vo3 r]; intros vo2 vo1; cbn; try easy.
-  case_var_zero vo2.
-  - rewrite
-      transpose_push_normalized_pushes_cons_raw_closing; cbn.
-    rewrite transpose_push_push_zero_left; cbn.
-    rewrite transpose_push_reducing_push_pop; easy.
-  - rewrite
-      transpose_push_normalized_pushes_cons_raw_closing; cbn.
-    case_var_zero vo1.
-    + destruct vo2; easy.
-    + rewrite
-        transpose_push_normalized_pushes_cons_raw_closing;
-        cbn; reduce_var_zero.
-      rewrite <- transpose_pushes_reverse_left.
-      rewrite transpose_push_raw_closing_reverse_right.
-      rewrite transpose_push_raw_closing_reverse_middle.
+  generalize dependent v1.
+  generalize dependent v2.
+  induction r as [|vl r IHr vr]; intros v2 v1; cbn; try easy.
+  case_vars_eq v2 vl as Heq1 Hneq1.
+  - rewrite var_eqb_false
+      by apply irreducible_transposed_1; cbn.
+    rewrite var_eqb_true
+      by apply transpose_reducible_push_pop.
+    rewrite reducible_transposed_2
+      with (v2 := v2) (v1 := v1) by easy.
+    easy.
+  - case_vars_eq (shift_var v2 v1) vl as Heq2 Hneq2.
+    + apply reducible_transposed_2 in Heq2 as Heq3;
+        reduce_vars.
+      rewrite <- transpose_reducible_push_pop.
+      easy.
+    + apply irreducible_transposed_3 in Hneq2 as Hneq3;
+        try easy; reduce_vars.
+      rewrite var_eqb_false
+        by (apply transpose_irreducible_push_pop; easy).
+      rewrite transpose_push_push_pop_reverse_left.
       rewrite IHr.
-      rewrite transpose_push_push_pop_zero_reverse_middle.
-      rewrite transpose_push_push_pop_zero_reverse_right
-        by easy.
+      rewrite <- transpose_pushes_reverse_left
+        with (v3 := vr).
+      rewrite transpose_push_raw_renaming_reverse_right.
+      rewrite transpose_push_raw_renaming_reverse_middle.
+      rewrite transpose_push_push_pop_reverse_middle.
+      rewrite transpose_push_push_pop_reverse_right
+        by congruence.
       easy.
 Qed.
 
-Lemma transpose_push_compose_raw_closing_push r1 r2 vo :
-  transpose_push_raw_closing_push
-    vo (compose_raw_closing r1 r2)
-  = transpose_push_raw_closing_push
-      (transpose_push_raw_closing_push vo r1) r2.
+Lemma transpose_push_compose_raw_renaming_push r1 r2 v :
+  transpose_push_raw_renaming_push
+    v (compose_raw_renaming r1 r2)
+  = transpose_push_raw_renaming_push
+      (transpose_push_raw_renaming_push v r1) r2.
 Proof.
-  generalize dependent vo.
+  generalize dependent v.
   generalize dependent r2.
-  induction r1 as [|vo' r1]; intros r2 vo; cbn; try easy.
-  rewrite rhs_push_transpose_push_raw_closing,
-    rhs_raw_closing_transpose_push_raw_closing.
-  rewrite transpose_push_normalized_pushes_cons_push; cbn.
-  case_var_zero vo; try easy.
+  induction r1 as [|vl r1 IHr1 vr]; intros v2 v1; cbn; try easy.
+  rewrite rhs_push_transpose_push_raw_renaming,
+    rhs_raw_renaming_transpose_push_raw_renaming.
+  case_vars_eq v1 vl; try easy.
   rewrite IHr1.
-  apply transpose_push_raw_closing_reverse_right.
+  apply transpose_push_raw_renaming_reverse_right.
 Qed.
 
-Lemma transpose_push_compose_raw_closing_raw_closing r1 r2 vo :
-  normalized_pushes r2 ->
-  transpose_push_raw_closing_raw_closing
-    vo (compose_raw_closing r1 r2)
-  = compose_raw_closing
-      (transpose_push_raw_closing_raw_closing vo r1)
-      (transpose_push_raw_closing_raw_closing
-         (transpose_push_raw_closing_push vo r1) r2).
+Lemma transpose_push_compose_raw_renaming_raw_renaming r1 r2 v :
+  transpose_push_raw_renaming_raw_renaming
+    v (compose_raw_renaming r1 r2)
+  = compose_raw_renaming
+      (transpose_push_raw_renaming_raw_renaming v r1)
+      (transpose_push_raw_renaming_raw_renaming
+         (transpose_push_raw_renaming_push v r1) r2).
 Proof.
-  generalize dependent vo.
+  generalize dependent v.
   generalize dependent r2.
-  induction r1 as [|vo' r1]; intros r2 vo Hnorm; cbn; try easy.
-  rewrite rhs_push_transpose_push_raw_closing,
-    rhs_raw_closing_transpose_push_raw_closing.
-  rewrite
-    transpose_push_normalized_pushes_cons_raw_closing; cbn.
-  case_var_zero vo; try easy.
-  rewrite IHr1;
-    try (apply transpose_push_raw_closing_raw_closing_normalized;
-         easy).
-  rewrite transpose_push_raw_closing_reverse_left.
-  rewrite transpose_push_compose_raw_closing_push.
-  rewrite transpose_push_raw_closing_reverse_middle.
-  rewrite compose_normalized_pushes_cons;
-    try (apply transpose_push_raw_closing_raw_closing_normalized;
-         easy); cbn.
-  rewrite rhs_push_transpose_push_raw_closing,
-    rhs_raw_closing_transpose_push_raw_closing.
+  induction r1 as [|vl r1 IHr1 vr]; intros r2 v; cbn; try easy.
+  rewrite rhs_push_transpose_push_raw_renaming,
+    rhs_raw_renaming_transpose_push_raw_renaming.
+  case_vars_eq v vl; try easy.
+  rewrite IHr1.
+  rewrite transpose_push_raw_renaming_reverse_left.
+  rewrite transpose_push_compose_raw_renaming_push.
+  rewrite transpose_push_raw_renaming_reverse_middle.
+  rewrite rhs_push_transpose_push_raw_renaming,
+    rhs_raw_renaming_transpose_push_raw_renaming.
   easy.
 Qed.
 
-Lemma raw_closing_associative r1 r2 r3 :
-  normalized_pushes r3 ->
-  compose_raw_closing r1 (compose_raw_closing r2 r3)
-  = compose_raw_closing (compose_raw_closing r1 r2) r3.
+Lemma raw_renaming_associative r1 r2 r3 :
+  compose_raw_renaming r1 (compose_raw_renaming r2 r3)
+  = compose_raw_renaming (compose_raw_renaming r1 r2) r3.
 Proof.
   generalize dependent r2.
   generalize dependent r3.
-  induction r1; cbn; intros r3 r2 Hnorm; try easy.
-  rewrite compose_normalized_pushes_cons by easy; cbn.
-  rewrite !rhs_push_transpose_push_raw_closing,
-    !rhs_raw_closing_transpose_push_raw_closing.
-  rewrite transpose_push_compose_raw_closing_raw_closing
-    by easy.
-  rewrite IHr1
-    by (apply transpose_push_raw_closing_raw_closing_normalized;
-        easy).
-  rewrite transpose_push_compose_raw_closing_push.
+  induction r1; cbn; intros r3 r2; try easy.
+  rewrite !rhs_push_transpose_push_raw_renaming,
+    !rhs_raw_renaming_transpose_push_raw_renaming.
+  rewrite transpose_push_compose_raw_renaming_raw_renaming.
+  rewrite IHr1.
+  rewrite transpose_push_compose_raw_renaming_push.
   easy.
 Qed.
 
-Lemma closing_associative r1 r2 r3 :
-  compose_closing r1 (compose_closing r2 r3)
-  = compose_closing (compose_closing r1 r2) r3.
+(* Composition of matching extensions *)
+
+Lemma compose_raw_renaming_extend v1 r1 v2 r2 v3 :
+  compose_raw_renaming
+    (raw_renaming_extend v1 r1 v2)
+    (raw_renaming_extend v2 r2 v3)
+  = raw_renaming_extend v1 (compose_raw_renaming r1 r2) v3.
 Proof.
-  destruct r1, r2, r3.
-  apply lift_closing_eq; cbn.
-  apply raw_closing_associative; easy.
+  cbn; rewrite var_eqb_true by easy; cbn.
+  easy.
+Qed.
+
+(* [apply_raw_renaming] is a semigroup action *)
+
+Definition apply_renaming_rhs_var r : var_op 0 1 :=
+  lift_var_op (apply_raw_renaming_var (rhs_raw_renaming r))
+  @ push_var (rhs_push r).
+Arguments apply_renaming_rhs_var r /.
+
+Lemma apply_transpose_push_raw_renaming v r :
+  push_var v
+  @ apply_raw_renaming_var r
+  =v=
+  apply_renaming_rhs_var (transpose_push_raw_renaming v r).
+Proof.
+  generalize dependent v.
+  induction r as [|vl r IHr vr]; intros v; cbn.
+  - simplify_var_ops; easy.
+  - case_vars_eq v vl.
+    + rewrite push_pop_identity'; easy.
+    + rewrite transpose_push_pop' by easy.
+      simplify_var_ops.
+      rewrite <- lift_var_op_compose'.
+      rewrite IHr; cbn; simplify_var_ops.
+      rewrite transpose_swap_lifted'.
+      rewrite transpose_pushes.
+      rewrite swap_swap_identity'.
+      easy.
+Qed.
+
+Lemma apply_compose_raw_renaming r1 r2 :
+  apply_raw_renaming_var (compose_raw_renaming r1 r2)
+  =v= apply_raw_renaming_var r1 @ apply_raw_renaming_var r2.
+Proof.
+  generalize dependent r2.
+  induction r1 as [|vl r1 IHr1 vr]; intros r2; cbn; try easy.
+  rewrite IHr1; simplify_var_ops.
+  rewrite apply_transpose_push_raw_renaming.
+  easy.
+Qed.
+
+Lemma apply_compose_raw_renaming' {N} r1 r2 (op : var_op N 0) :
+  apply_raw_renaming_var (compose_raw_renaming r1 r2) @ op
+  =v= apply_raw_renaming_var r1
+      @ (apply_raw_renaming_var r2 @ op).
+Proof.
+  rewrite apply_compose_raw_renaming, var_op_associative.
+  easy.
+Qed.
+
+Lemma apply_inverse_raw_renaming_left r :
+  apply_raw_renaming_var (inverse_raw_renaming r)
+  @ apply_raw_renaming_var r
+  =v= 1.
+Proof.
+  induction r as [|vl r IHr vr];
+    cbn; try easy; simplify_var_ops.
+  rewrite push_pop_identity'.
+  rewrite <- lift_var_op_compose'.
+  rewrite IHr; simplify_var_ops.
+  rewrite pop_push_identity.
+  easy.
+Qed.
+
+Lemma apply_inverse_raw_renaming_left' {N} r (op : var_op N 0) :
+  apply_raw_renaming_var (inverse_raw_renaming r)
+  @ (apply_raw_renaming_var r @ op)
+  =v= op.
+Proof.
+  rewrite var_op_associative, apply_inverse_raw_renaming_left,
+    var_op_left_identity.
+  easy.
+Qed.
+
+Lemma apply_inverse_raw_renaming_right r :
+  apply_raw_renaming_var r
+  @ apply_raw_renaming_var (inverse_raw_renaming r)
+  =v= 1.
+Proof.
+  induction r as [|vl r IHr vr];
+    cbn; try easy; simplify_var_ops.
+  rewrite push_pop_identity'.
+  rewrite <- lift_var_op_compose'.
+  rewrite IHr; simplify_var_ops.
+  rewrite pop_push_identity.
+  easy.
+Qed.
+
+Lemma apply_inverse_raw_renaming_right' {N} r (op : var_op N 0) :
+  apply_raw_renaming_var r
+  @ (apply_raw_renaming_var (inverse_raw_renaming r) @ op)
+  =v= op.
+Proof.
+  rewrite var_op_associative, apply_inverse_raw_renaming_right,
+    var_op_left_identity.
+  easy.
+Qed.
+
+(* Define equivalence of [raw_renaming] in terms of
+   [apply_raw_renaming] *)
+
+Definition equivalent_raw_renaming : relation raw_renaming :=
+  fun r1 r2 =>
+    apply_raw_renaming_var r1
+    =v= apply_raw_renaming_var r2.
+
+Notation "r1 =rr= r2" :=
+  (equivalent_raw_renaming r1 r2) (at level 70).
+
+Instance equivalent_raw_renaming_equiv :
+  Equivalence equivalent_raw_renaming.
+Proof.
+  apply @Build_Equivalence; try easy.
+  intros op1 op2 op3 Heq1 Heq2 v.
+  rewrite Heq1, Heq2; easy.
+Qed.
+
+Add Parametric Morphism : raw_renaming_extend
+    with signature eq ==> equivalent_raw_renaming ==> eq
+                     ==> equivalent_raw_renaming
+      as raw_renaming_extend_mor.
+  unfold equivalent_raw_renaming; intros * Heq *; cbn.
+  rewrite Heq; easy.
+Qed.
+
+Add Parametric Morphism : apply_raw_renaming_var
+    with signature equivalent_raw_renaming ==> @eq_var_op 0 0
+      as apply_raw_renaming_var_mor.
+  intros * Heq v; rewrite Heq; easy.
+Qed.
+
+Add Parametric Morphism : compose_raw_renaming
+    with signature equivalent_raw_renaming
+                     ==> equivalent_raw_renaming
+                     ==> equivalent_raw_renaming
+      as compose_raw_renaming_mor.
+  intros * Heq1 * Heq2; unfold equivalent_raw_renaming.
+  rewrite! apply_compose_raw_renaming; cbn.
+  rewrite Heq1, Heq2; easy.
+Qed.
+
+Add Parametric Morphism : inverse_raw_renaming
+    with signature equivalent_raw_renaming
+                     ==> equivalent_raw_renaming
+      as inverse_raw_renaming_mor.
+  unfold equivalent_raw_renaming; intros * Heq.
+  rewrite <- apply_inverse_raw_renaming_left'.
+  rewrite <- Heq.
+  rewrite apply_inverse_raw_renaming_right.
+  easy.
+Qed.
+
+(* Under this equivalence raw_renamings form a group *)
+
+Lemma raw_renaming_left_inverse r :
+  compose_raw_renaming (inverse_raw_renaming r) r
+  =rr= raw_renaming_id.
+Proof.
+  unfold equivalent_raw_renaming.
+  rewrite apply_compose_raw_renaming.
+  rewrite apply_inverse_raw_renaming_left.
+  easy.
+Qed.
+
+Lemma raw_renaming_right_inverse r :
+  compose_raw_renaming r (inverse_raw_renaming r)
+  =rr= raw_renaming_id.
+Proof.
+  unfold equivalent_raw_renaming.
+  rewrite apply_compose_raw_renaming.
+  rewrite apply_inverse_raw_renaming_right.
+  easy.
+Qed.
+
+(* Extensions can be reordered under the equivalence *)
+
+Lemma swap_raw_renaming_extend v1 v2 r v3 v4 :
+  raw_renaming_extend
+    v1 (raw_renaming_extend v2 r v3) v4
+  =rr= raw_renaming_extend
+         (shift_var v1 v2)
+         (raw_renaming_extend
+            (unshift_var v2 v1) r (unshift_var v3 v4))
+         (shift_var v4 v3).
+Proof.
+  unfold equivalent_raw_renaming; cbn; simplify_var_ops.
+  rewrite transpose_pops', transpose_pushes,
+    transpose_swap_lifted', swap_swap_identity'.
+  easy.
 Qed.
